add conditions

Roos/chomsky_schuetzenberger.thy
@@ -53,6 +53,40 @@ assumes \<open>CFL.cfl TYPE('a) L\<close>
 shows \<open>\<exists>P S::'a. L = Lang P S \<and> (\<forall>p \<in> P. CNF_rule p)\<close> (* TODO Startsymbol nicht auf rechter Seite?*)
 sorry
 
+(* (Directly) After each (Cl,p,1) always comes a (Op,p,2)*)
+definition P1 :: \<open>('a \<times> ('a, 'b) sym list) set \<Rightarrow> (bracket \<times> ('a \<times> ('a, 'b) sym list) \<times> nat) list \<Rightarrow> bool\<close> where
+\<open>P1 P x = (\<forall>p \<in> P. \<forall> i < length x.
+  x ! i = (Cl, (p, 1)) \<longrightarrow> ( i+1 < length x \<and> x ! (i+1) = (Op, (p, 2))))\<close>
+
+(*After any (Cl,pi,2) there never comes an (Op,...) *)
+definition P2 :: \<open>('a \<times> ('a, 'b) sym list) set \<Rightarrow> (bracket \<times> ('a \<times> ('a, 'b) sym list) \<times> nat) list \<Rightarrow> bool\<close> where
+\<open>P2 P x = (\<forall>p \<in> P. \<forall>r. (\<forall>i j. i < length x \<and> j < length x \<and> i < j \<and> x ! i = (Cl, (p, 2)) \<longrightarrow> x ! j \<noteq> (Op, r)))\<close>
+
+(*If pi = A\<rightarrow>BC, then after each (Op,pi,1) always comes a (Op,p,1) where B = lhs of p And after each (Op,pi,2) always comes a (Op,sigma,1) where C = lhs of sigma *)
+definition P3 :: \<open>(bracket \<times> ('a \<times> ('a, 'b) sym list) \<times> nat) list \<Rightarrow> bool\<close> where
+\<open>P3 x = (\<forall>i < length x. 
+       (\<exists>A B C. x ! i = (Op, ((A, [Nt B, Nt C]), 1)) \<longrightarrow> 
+          ((i+1) < length x \<and> (\<exists>p l. x ! (i+1) = (Op, (p, 1)) \<and> p = (B, l)))) \<and>
+       (\<exists>A B C. x ! i = (Op, ((A, [Nt B, Nt C]), 2)) \<longrightarrow> 
+          ((i+1) < length x \<and> (\<exists>\<sigma> l. x ! (i+1) = (Op, (\<sigma>, 1)) \<and> \<sigma> = (C, l)))))\<close>
+
+
+(*If pi = A\<rightarrow>a then after each (Op,pi,1) comes a (Cl,pi,1) and after each (Op,pi,2) comes a (Cl,pi,2) *)
+definition P4 :: \<open>(bracket \<times> ('a \<times> ('a, 'b) sym list) \<times> nat) list \<Rightarrow> bool\<close> where
+\<open>P4 x = ((\<forall>i < length x - 1. 
+        (\<exists>A a. x ! i = (Op, ((A, [Tm a]), 1)) \<longrightarrow> x ! (i + 1) = (Cl, ((A, [Tm a]), 1))) \<and>
+        (\<exists>A a. x ! i = (Op, ((A, [Tm a]), 2)) \<longrightarrow> x ! (i + 1) = (Cl, ((A, [Tm a]), 2)))))\<close>
+
+(*For all A, if A produces x under P', then there eists some pi \<in> P with lhs A such that x begins with (Op,pi,1) *)
+definition P5 :: \<open>('a \<times> ('a, 'b) sym list) set \<Rightarrow> 'a \<Rightarrow> (bracket \<times> ('a \<times> ('a, 'b) sym list) \<times> nat) list \<Rightarrow> bool\<close> where
+\<open>P5 P A x = (( (\<forall>w. derives (image transform_production P) [Nt A] w) \<longrightarrow> 
+       (\<exists>\<pi> l. \<pi> \<in> P \<and> \<pi> = (A, l) \<and> x \<noteq> [] \<and> x ! 0 = (Op, \<pi>, 1))))\<close>
+
+definition Re :: \<open>('a \<times> ('a, 'b) sym list) set \<Rightarrow> 'a \<Rightarrow> (bracket \<times> ('a \<times> ('a, 'b) sym list) \<times> nat) list set\<close> where
+\<open>Re P A = {x::(bracket \<times> ('a \<times> ('a, 'b) sym list) \<times> nat) list. 
+(P1 P x) \<and> (P2 P x) \<and> (P3 x) \<and> (P4 x) \<and> (P5 P A x)}\<close>
+
+
 (* Unser gewünschtes Resultat *)
 lemma chomsky_schuetzenberger :
 assumes \<open>CFL.cfl TYPE('a) L\<close> 
@@ -62,15 +96,17 @@ proof -
 have \<open>\<exists>P S::'a. L = Lang P S \<and> (\<forall>p \<in> P. CNF_rule p)\<close> using \<open>cfl TYPE('a) L\<close> CNF_existence by auto
 then obtain P where \<open>\<exists>S::'a. L = Lang P S \<and> (\<forall>p \<in> P. CNF_rule p)\<close> by blast
 then obtain S where \<open>L = Lang P S\<close> and \<open>(\<forall>p \<in> P. CNF_rule p)\<close> by blast (* Warum geht das nicht in einzer Zeile...?*)
-
+term P
 let ?\<Gamma> = \<open>P \<times> {1::nat,2}\<close>
 let ?P' = \<open>image transform_production P\<close>
 let ?L' = \<open>Lang ?P' S\<close>
+term ?L'
 
-have \<open>?L' \<subseteq> dyck_language ?\<Gamma>\<close> sorry
+have \<open>?L' \<subseteq> dyck_language ?\<Gamma>\<close> sorry (* evtl unnötig? *)
 
-
-
+have \<open>\<forall>A. \<forall>x::(bracket \<times> ('a \<times> ('a, 'b) sym list) \<times> nat) list. 
+(image transform_production P) \<turnstile> [Nt S] \<Rightarrow>* (map Tm x) \<longleftrightarrow> x \<in> (dyck_language ?\<Gamma>) \<inter> (Re P A)\<close> sorry
+then have \<open>?L' = (dyck_language ?\<Gamma>) \<inter> (Re P S)\<close> by (metis (no_types, lifting) CFG.Lang_def mem_Collect_eq subsetI subset_antisym)
 
 qed
 
